tensor product
$$
(\bold a \otimes \bold b)\bold c = (\bold b \cdot \bold c)\bold a
$$
skewsymmetric
$$
sym(A) = \frac{1}{2}(\bold A + \bold 
A^T) \qquad skw(\bold A) = \frac{1}{2}(\bold A - \bold A^T)
$$

$$
ax(\bold C)\times \bold b = \bold C \bold b \qquad skewt(\bold c)\bold b = \bold c \times \bold b
$$

 并且
$$
\bold g_1 = \bold A \bold f_1 \qquad \bold g_2 = \bold A \bold f_2 \qquad \bold g_3 = \bold A \bold f_3 \\
\bold A = \bold g_1 \otimes \bold f_1 + \bold g_2 \otimes \bold f_2 + \bold g_3 \otimes \bold f_3
$$
===========An Introduction to Physically Based Modeling: Rigid Body Simulation I—Unconstrained Rigid Body Dynamics  

if a and b are 3 -vectors then a \times b is
$$
a^*b = \begin{bmatrix} 0 & -a_z & a_y \\ a_z & 0 & -a_x \\ -a_y & a_x & 0\end{bmatrix}\begin{bmatrix} b_x \\ b_y \\ b_z\end{bmatrix} = \begin{bmatrix} a_yb_z - b_ya_z \\ a_zb_x - a_xb_z \\ a_xb_y - b_xa_y\end{bmatrix} = a\times b
$$
同样rotation 也可以将叉乘化为矩阵乘法

double cross product, a, b and c are vectors
$$
\bold a \times (\bold b \times \bold c) = (\bold a \cdot \bold c)\bold b - (\bold a \cdot \bold b)\bold c
$$
Another
$$
\bold a \times (\bold b \times \bold c) + \bold b \times (\bold c \times \bold a) + \bold c \times (\bold a \times \bold b) = \bold 0
$$
并且
$$
(\bold a \times \bold b)\cdot \bold c = det\begin{bmatrix} a_x & b_x & c_x \\ a_y & b_y & c_y \\ a_z & b_z & c_z\end{bmatrix}
$$
也就是
$$
(\bold a \times \bold b)\cdot \bold c = (\bold b \times \bold c) \cdot \bold a = (\bold c \times \bold a)\cdot \bold b
$$
