Engineer Mechanics 3
$$
(\bold r_i \times m_i \bold v_i)' = \bold r_i \times \bold F_i + \sum_j \bold r_i \times \bold F_{ij}
$$
total moment of the external forces remain
$$
\bold M(0) = \sum_i \bold M_i^{(0)} = \sum_i r_i \times \bold F_i
$$
total angular momentum of the system
$$
\bold L(0) = \sum_i \bold L^{(0)}_i = \sum_i (\bold r_i \times m_i \bold v_i)
$$
然后就是angular momentum theorem
$$
\dot {\bold L}^{(0)} = \bold M^{(0)}
$$
\角动量的变化速率等于外部的moment，又
$$
L_{iz} = m_i r_i^2 \dot \varphi \qquad L_z = \sum_i m_i r_i^2 \dot \varphi = \Theta \dot \varphi \qquad \Theta_a \ddot \varphi = M
$$
Theta is the mass moment of inertia

 elastic collision
$$
\overline v_1 = \frac{m_1v_1 + m_2v_2 - em_2(v_1 - v_2)}{m_1 + m_2}\\
\overline v_2 = \frac{m_1v_1 + m_2v_2 + em_1(v_1 + v_2)}{m_1 + m_2}
$$
thrust T = - mu w. mu is the rate of change of the mass. w is the increasing velocity.
$$
m(t)\dot v = -m(t)g + T \qquad \frac{dv}{dt} = -g - \frac{1}{m}\frac{dm}{dt}w
$$
也就是
$$
m(t) = m_I - \mu t \qquad \dot m = - \mu \qquad v(t) = w\ln \frac{m_I}{m_I - \mu t} - gt 
$$
